examples/sgx/Util.fst
@@ -6,3 +6,37 @@ let u64 = UInt64.t
 
 val cast_to_nat: u64 -> nat
 let cast_to_nat  i = 0
+
+(*
+  Bitmap layout
+	 	_____________________
+		| 8-bytes /64-bits   |
+		+____________________+
+bitmapstart->	|bbbbbbb.......bbbbb |
+		+____________________+
+bitmapoffset->	|bbbbbbb.......bbbbb |
+		|  |    	     |
+		|  idx    	     |
+		+____________________+
+
+ Each entry is a 8 bytes long and each bit represents if the corresponding 64-bytes at an 
+ address(computed by the formula below) is writable.
+Each offset represents the bit array for 64 64-bit addresses.
+ 
+ To obtain address represented index 'idx' at 'bitmapoffset' is given as:
+	address = ((bitmapoffset * 64) + idx) + enclave_start_address
+
+ To check if 'addr' is writable, compute the index 'idx' as follows:
+	bitmapoffset  = (addr - enclave_start_address) / 64
+	idx 	      = (addr - enclave_start_address) % 64
+*)
+
+val get_address_represented_in_bitmap:nat->nat->nat->nat
+let get_address_represented_in_bitmap base bitmapstart addr = 
+	let bitmapoffset = (addr - bitmapstart) in
+	let tmp = (op_Multiply bitmapoffset 64) in
+	(* Not including index, since a store can operate only on 8byte granularity
+	  Optimize it later to get precise address
+	*)
+	let addroffset = (tmp+base) in
+	 addroffset
